add wpgen

Lgtm/Hyper/WP.lean
@@ -8,8 +8,6 @@ import Lgtm.Unary.WP
 
 import Lean
 
-
-
 import Lgtm.Hyper.HProp
 import Lgtm.Hyper.YSimp
 import Lgtm.Hyper.YChange
@@ -27,23 +25,23 @@ local notation "htrm" => htrm α
 local notation "hval" => hval α
 local notation "hhProp" => hhProp α
 
-/- ---------- Definition and Structural Rules for [wp] ---------- -/
+/- ---------- Definition and Structural Rules for [hwp] ---------- -/
 
-/- Definition of [wp] -/
+/- Definition of [hwp] -/
 
 
 def hwp (ht : htrm) (Q : hval -> hhProp) : hhProp := (heval s · ht Q)
 
-/- Equivalence b/w [wp] and [triple] -/
+/- Equivalence b/w [hwp] and [triple] -/
 
 lemma hwp_equiv : H ==> hwp s ht Q = htriple s ht H Q := by rfl
 
-/- Consequence rule for [wp] -/
+/- Consequence rule for [hwp] -/
 lemma hwp_conseq (ht : htrm) (Q Q' : hval -> hhProp) :
   Q ===> Q' -> hwp s ht Q ==> hwp s ht Q' := by
   sby move=> ???/=; apply heval_conseq
 
-/- Frame rule for [wp] -/
+/- Frame rule for [hwp] -/
 
 lemma hwp_frame (ht : htrm) (Q : hval -> hhProp) (H : hhProp) :
   hwp s ht Q ∗ H ==> hwp s ht (Q ∗ H) := by
@@ -137,6 +135,203 @@ lemma hwp_seq (ht₁ ht₂ : htrm) (Q : hval -> hhProp) :
 lemma hwp_let (x : α -> var) (ht₁ ht₂ : htrm) (Q : hval -> hhProp) :
   hwp s ht₁ (fun v ↦ hwp s (fun a => subst (x a) (v a) (ht₂ a)) Q) ==> hwp s (fun a => trm_let (x a) (ht₁ a) (ht₂ a)) Q :=
   by sby move=> ??; apply heval_let
+
+
+/- ------------------ Definition of [hwpgen] ------------------ -/
+
+/- Defining [hmkstruct] -/
+
+abbrev hformula := (hval -> hhProp) -> hhProp
+
+local notation "hformula" => @hformula α
+
+def hmkstruct (F : hformula) :=
+  fun (Q : hval -> hhProp) => h∃ Q' : hval -> hhProp, F Q' ∗ (Q' -∗ Q)
+
+def hstructural (F : hformula) := forall Q, F Q ==> hmkstruct F Q
+
+def hstructuralPred (F : β -> hformula) := ∀ x, hstructural (F x)
+
+def hwpgen_fail : hformula := fun _ => ⌜False⌝
+
+def hwpgen_val  (v : hval) : hformula := (· v)
+
+abbrev ctx (α : Type) := AList (fun _ : var ↦ α -> val)
+
+def hwpgen_var (E : ctx α) (vr : var) : hformula := fun Q =>
+  match AList.lookup vr E with
+  | some hv => hwpgen_val hv Q
+  | _ => ⌜False⌝
+
+@[simp]
+def hwpgen_varE :
+  hwpgen_var (E : ctx α) y =
+    (match AList.lookup y E with
+     | .some hv => hwpgen_val hv
+     | _ => fun _ => ⌜False⌝)
+    := by
+  unfold hwpgen_var=> !? /=
+  scase: (AList.lookup y E)=> //
+    -- if y ∈ E then hwpgen_val  else hwpgen_fail := by
+
+def hwpgen_fun (s : Set α) (Fof : hval → hformula) : hformula :=
+  fun Q ↦ h∀ vf, ⌜forall vx Q', Fof vx Q' ==>
+    hwp s (fun a => trm_app (trm_val $ vf a) (trm_val $ vx a)) Q'⌝ -∗ Q vf
+
+def hwpgen_fix (s : Set α) (Fof : hval -> hval → hformula) : hformula :=
+  fun Q ↦ h∀ vf, ⌜forall vx Q', Fof vf vx Q' ==>
+    hwp s (fun a => trm_app (trm_val $ vf a) (trm_val $ vx a)) Q'⌝ -∗ Q vf
+
+
+def hwpgen_seq (F₁ F₂ : hformula) : hformula :=
+  fun Q ↦ F₁ (fun _ ↦ F₂ Q)
+
+
+def hwpgen_let (F₁ : hformula) (F₂of : hval -> hformula) : hformula :=
+  fun Q ↦ F₁ (fun v ↦ F₂of v Q)
+
+def hwpgen_if (t : htrm) (F₁ F₂ : hformula) : hformula :=
+  fun Q ↦ h∃ b : Bool, ⌜t = fun _ => trm_val b⌝ ∗ (if b then F₁ Q else F₂ Q)
+
+def hwpgen_if_trm (F₀ F₁ F₂ : hformula) : hformula := hwpgen_let F₀ (fun v => hmkstruct $ hwpgen_if (trm_val ∘ v) F₁ F₂)
+
+def hwpgen_app (s : Set α) (t : htrm) : hformula := fun Q => h∃ H, H ∗ ⌜htriple s t H Q⌝
+
+def hwpgen_for (v₁ v₂ : htrm) (F1 : hval -> hformula) : hformula :=
+  hmkstruct fun Q =>
+    h∃ n₁ n₂ : Int, ⌜v₁ = fun _ => trm_val n₁⌝ ∗ ⌜v₂ = fun _ => trm_val n₂⌝ ∗
+      h∀ (S : Int -> hformula),
+        (let F i :=
+          if i < n₂ then
+            hwpgen_seq (F1 (fun _ => val_int i)) (S (i + 1))
+          else hwpgen_val fun _ => val_unit
+        ⌜hstructuralPred S /\ ∀ i, F i ===> S i⌝ -∗ S n₁ Q )
+
+def wpgen_while (F1 F2 : hformula) : hformula := hmkstruct fun Q =>
+  h∀ R : hformula,
+    let F := hwpgen_if_trm F1 (hwpgen_seq F2 R) (hwpgen_val fun _ => val_unit)
+    ⌜hstructural R ∧ F ===> R⌝ -∗ R Q
+
+@[simp]
+abbrev isubst (E : ctx α) (a : α) (t : trm) : trm :=
+  match t with
+  | trm_val v =>
+      v
+  | trm_var x =>
+      match AList.lookup x E with
+      | none   => t
+      | some v => v a
+  | trm_fun x t1 =>
+      trm_fun x (isubst (AList.erase x E) a t1)
+  | trm_fix f x t1 =>
+      trm_fix f x (isubst (AList.erase x (AList.erase f E)) a t1)
+  | trm_if t0 t1 t2 =>
+      trm_if (isubst E a t0) (isubst E a t1) (isubst E a t2)
+  | trm_seq t1 t2 =>
+      trm_seq (isubst E a t1) (isubst E a t2)
+  | trm_let x t1 t2 =>
+      trm_let x (isubst E a t1) (isubst (AList.erase x E) a t2)
+  | trm_app t1 t2 =>
+      trm_app (isubst E a t1) (isubst E a t2)
+  | trm_for x n1 n2 t =>
+      trm_for x (isubst E a n1) (isubst E a n2) (isubst (AList.erase x E) a t)
+  | trm_while c t =>
+      trm_while (isubst E a c) (isubst E a t)
+
+@[simp]
+lemma isubst0 : isubst (∅ : ctx α) = fun _ x => x := by sorry
+
+@[simp]
+lemma subst_isubst (v : hval) (t : htrm) :
+  (fun a => subst x (v a) (isubst (AList.erase x E) a (t a))) =
+  fun a => isubst (AList.insert x v E) a (t a) := by sorry
+
+
+class HWpSound (s : Set α) (t : htrm) (E : ctx α) (F : outParam hformula) :=
+  impl : ∀ Q, F Q ==> hwp s (fun a => isubst E a (t a)) Q
+
+@[instance 0]
+instance : HWpSound (s : Set α) t (∅ : ctx α) (hwp s t) := ⟨by sby srw isubst0⟩
+
+instance : HWpSound s (fun a => trm_val (hv a)) E (hwpgen_val hv) := ⟨by sby move=> ? /==; apply htriple_val⟩
+instance : HWpSound s (fun _ => trm_var hr) E (hwpgen_var E hr) :=
+  ⟨by move=> ? /==
+      scase: (AList.lookup hr E)=> /==
+      { ysimp=> // }
+      move=> ?; apply htriple_val=> //⟩
+
+@[simp]
+lemma hWpSoundTriple {inst: HWpSound s t E F} Q : htriple s (fun a => isubst E a (t a)) (F Q) Q = true := by
+  simp; apply inst.impl
+
+@[simp]
+lemma hWpSoundWp {inst: HWpSound s t E F} Q : (F Q) ==> hwp s (fun a => isubst E a (t a)) Q = true := by
+  simp; apply inst.impl
+
+instance [inst: HWpSound s t₁ E F₁] [HWpSound s t₂ E F₂] :
+  HWpSound s (fun a => trm_if (t₀ a) (t₁ a) (t₂ a)) E (hwpgen_if t₀ F₁ F₂) := ⟨by
+  -- sby
+    move=> ?; srw hwpgen_if; ysimp=> b; scase_if=> ? /== <;> apply htriple_if=> /==⟩
+
+lemma hwp_sound_conseq (F : hformula) :
+  F Q ==> hwp s t Q ->
+  Q ===> Q' ->
+  F Q ==> hwp s t Q' := by
+    move=> ??
+    sby ychange hwp_conseq
+
+instance [HWpSound s t₁ E F₁] [HWpSound s t₂ E F₂] :
+  HWpSound s (fun a => trm_seq (t₁ a) (t₂ a)) E (hwpgen_seq F₁ F₂) := ⟨by
+  move=> Q /==; ychange hwp_seq
+  srw hwpgen_seq; apply hwp_sound_conseq=> // ? //⟩
+
+instance {F₂ : hval -> hformula} {x : var} {t₂ : htrm}
+  [HWpSound s t₁ E F₁]
+  [inst: ∀ hv, HWpSound s t₂ (E.insert x hv) (F₂ hv)] :
+  HWpSound s (fun a => trm_let x (t₁ a) (t₂ a)) E (hwpgen_let F₁ F₂) := ⟨by
+  move=> Q /==; ychange hwp_let
+  srw hwpgen_let; apply hwp_sound_conseq=> // ? //⟩
+  -- srw seq at inst
+  -- move=> Q; ychange hwp_let
+  -- srw hwpgen_let; apply hwp_sound_conseq=> // ? //⟩
+
+instance {t₁ t₂ : htrm} : HWpSound s (fun a => trm_app (t₁ a) (t₂ a)) E (hwpgen_app s (fun a => isubst E a $ trm_app (t₁ a) (t₂ a))) := ⟨by
+  sby move=> Q; srw hwpgen_app; ysimp⟩
+
+-- TODO: Add instance for `hwpgen_for` and `hwpgen_while`
+
+lemma hwp_of_hwpgen [inst: HWpSound s t ∅ F] :
+  H ==> F Q ->
+  H ==> hwp s t Q := by
+    move=> M; ychange M
+    shave->: t = fun a => isubst ∅ a $ t a
+    { srw isubst0 }
+    sby srw hWpSoundWp
+
+-- set_option  true
+example :
+  ⌜False⌝ ==> hwp {x : Int | x > 0} (fun i => [lang|
+    if i > 0 then
+       let x := 5 in
+       let y := 7 in
+       free (x + y);
+       y
+    else
+      y := x + 6;
+      6 + 7]) (fun _ => ⌜False⌝) := by
+  apply hwp_of_hwpgen=> /==; simp [AList.lookup]
+  ysimp=> //
+
+
+set_option trace.Meta.synthInstance true
+
+example :
+  ⌜False⌝ ==> hwp {x : Int | x > 0} (fun i => [lang|
+       let x := 5 in
+       let y := 7 in
+       x + y]) (fun _ => ⌜False⌝) := by
+  apply hwp_of_hwpgen
+  ysimp=> //
 
 
 end HWeakestPrecondition
